ictr_generic.fst
@@ -1,0 +1,51 @@
+module Ictr_generic
+
+open FStar.Seq
+open FStar.Ghost
+open Generic
+
+// the concrete state type
+// e.g. for the increment only counter (icounter), concrete_st = nat
+type concrete_st = nat
+
+// operation type
+// (the only operation is increment, so unit is fine)
+type op_t = unit
+
+// apply an operation to a state
+let do (s:concrete_st) (_:log_entry) : concrete_st = s + 1
+
+let rec lem_foldl (s:concrete_st) (l:log) 
+  : Lemma (ensures (seq_foldl do s l) = s + length l) (decreases length l)
+  = match length l with
+    |0 -> ()
+    |_ -> lem_foldl (do s (head l)) (tail l)
+
+//conflict resolution
+let resolve_conflict (x y:log_entry) : log =
+  cons x (cons y empty)
+
+let resolve_conflict_len (x y:log_entry)
+  : Lemma (Seq.length (resolve_conflict x y) = 2)
+  = ()
+
+let resolve_conflict_mem (x y:log_entry)
+  : Lemma (resolve_conflict_len x y;
+           let s = resolve_conflict x y in
+           (Seq.length s == 1 ==> is_x_or_y s x y) /\
+           (Seq.length s == 2 ==> is_x_and_y s x y))
+  = ()
+
+// concrete merge pre-condition
+let concrete_merge_pre (lca a b:concrete_st) : prop
+  = a >= lca /\ b >= lca
+
+// concrete merge operation
+let concrete_merge (lca:concrete_st) (cst1:concrete_st) (cst2:concrete_st{concrete_merge_pre lca cst1 cst2}) 
+  : concrete_st = cst1 + cst2 - lca
+
+let merge_prop (lca s1 s2:st)
+  : Lemma (requires v_of lca == init_of s1 /\
+                    init_of s1 == init_of s2) 
+          (ensures concrete_merge_pre (v_of lca) (v_of s1) (v_of s2)) =
+  admit()
